rustfrontend/RustIRown.v
@@ -524,7 +524,8 @@ Inductive step : state -> trace -> state -> Prop :=
     step (State f (Sstoragedead id) k le own m) E0 (State f Sskip k le own m)
          
 | step_call: forall f a al k le m vargs tyargs vf fd cconv tyres p orgs org_rels own1 own2
-    (TFEXPRLIST: move_place_list own1 (moved_place_list al) = own2), 
+    (TFEXPRLIST: move_place_list own1 (moved_place_list al) = own2)
+    (GFUN: good_function fd),
     classify_fun (typeof a) = fun_case_f tyargs tyres cconv ->
     eval_expr ge le m a vf ->
     eval_exprlist ge le m al tyargs vargs ->
@@ -532,6 +533,7 @@ Inductive step : state -> trace -> state -> Prop :=
     type_of_fundef fd = Tfunction orgs org_rels tyargs tyres cconv ->
     (* Cannot call drop glue *)
     (forall f', fd = Internal f' -> fn_drop_glue f' = None) ->
+    
     step (State f (Scall p a al) k le own1 m) E0 (Callstate vf vargs (Kcall p f le own2 k) m)
 
 | step_internal_function: forall vf f vargs k m e m' init_own
